src/Noninterference/FileDisk/TransferProofs.v
@@ -1,0 +1,181 @@
+Require Import Framework FileDiskLayer FileDiskRefinement FileDisk.RefinesSameOracle.RefinesSame FileDiskNoninterference FileDiskSSE.
+
+Theorem ss_AD_read:
+  forall n inum off u u',
+    SelfSimulation u 
+    (FileDisk.refinement.(Simulation.Definitions.compile) (FileDiskOp.(Op) (Read inum off))) 
+    (FileDisk.refinement.(Simulation.Definitions.compile) (FileDiskOp.(Op) (Read inum off))) 
+    (FileDisk.refinement.(Simulation.Definitions.compile) (FileDiskOp.(Op) Recover)) AD_valid_state 
+    (AD_related_states u' None) (eq u') (authenticated_disk_reboot_list n).
+Proof.
+    intros; eapply SS_transfer.
+    - apply ss_FD_read.
+    - apply read_simulation.
+    - apply read_simulation.
+    - apply abstract_oracles_exist_wrt_read.
+    - apply abstract_oracles_exist_wrt_read.
+    - apply ORS_read.
+    - unfold exec_compiled_preserves_validity,
+    refines_valid, FD_valid_state; intros; eauto.
+    - unfold exec_compiled_preserves_validity,
+    refines_valid, FD_valid_state; intros; eauto.
+    - unfold refines_related; apply SelfSimulation_Exists_read.
+Qed.
+
+Theorem ss_AD_write:
+  forall n inum off u u' v,
+    SelfSimulation u 
+    (FileDisk.refinement.(Simulation.Definitions.compile) (FileDiskOp.(Op) (Write inum off v))) 
+    (FileDisk.refinement.(Simulation.Definitions.compile) (FileDiskOp.(Op) (Write inum off v))) 
+    (FileDisk.refinement.(Simulation.Definitions.compile) (FileDiskOp.(Op) Recover)) AD_valid_state 
+    (AD_related_states u' None) (eq u') (authenticated_disk_reboot_list n).
+Proof.
+    intros; eapply SS_transfer.
+    - apply ss_FD_write.
+    - apply write_simulation.
+    - apply write_simulation.
+    - apply abstract_oracles_exist_wrt_write.
+    - apply abstract_oracles_exist_wrt_write.
+    - apply ORS_write.
+    - unfold exec_compiled_preserves_validity,
+    refines_valid, FD_valid_state; intros; eauto.
+    - unfold exec_compiled_preserves_validity,
+    refines_valid, FD_valid_state; intros; eauto.
+    - unfold refines_related; apply SelfSimulation_Exists_write.
+Qed.
+
+Theorem ss_AD_extend:
+  forall n inum u u' v,
+    SelfSimulation u 
+    (FileDisk.refinement.(Simulation.Definitions.compile) (FileDiskOp.(Op) (Extend inum v))) 
+    (FileDisk.refinement.(Simulation.Definitions.compile) (FileDiskOp.(Op) (Extend inum v))) 
+    (FileDisk.refinement.(Simulation.Definitions.compile) (FileDiskOp.(Op) Recover)) AD_valid_state 
+    (AD_related_states u' None) (eq u') (authenticated_disk_reboot_list n).
+Proof.
+    intros; eapply SS_transfer.
+    - apply ss_FD_extend.
+    - apply extend_simulation.
+    - apply extend_simulation.
+    - apply abstract_oracles_exist_wrt_extend.
+    - apply abstract_oracles_exist_wrt_extend.
+    - apply ORS_extend.
+    - unfold exec_compiled_preserves_validity,
+    refines_valid, FD_valid_state; intros; eauto.
+    - unfold exec_compiled_preserves_validity,
+    refines_valid, FD_valid_state; intros; eauto.
+    - unfold refines_related; apply SelfSimulation_Exists_extend.
+Qed.
+
+Theorem ss_AD_change_owner:
+  forall n inum u u' v,
+    SelfSimulation u 
+    (FileDisk.refinement.(Simulation.Definitions.compile) (FileDiskOp.(Op) (ChangeOwner inum v))) 
+    (FileDisk.refinement.(Simulation.Definitions.compile) (FileDiskOp.(Op) (ChangeOwner inum v))) 
+    (FileDisk.refinement.(Simulation.Definitions.compile) (FileDiskOp.(Op) Recover)) AD_valid_state 
+    (AD_related_states u' (Some inum)) (eq u') (authenticated_disk_reboot_list n).
+Proof.
+    intros; eapply SS_transfer.
+    - apply ss_FD_change_owner.
+    - apply change_owner_simulation.
+    - apply change_owner_simulation.
+    - apply abstract_oracles_exist_wrt_change_owner.
+    - apply abstract_oracles_exist_wrt_change_owner.
+    - apply ORS_change_owner.
+    - unfold exec_compiled_preserves_validity,
+    refines_valid, FD_valid_state; intros; eauto.
+    - unfold exec_compiled_preserves_validity,
+    refines_valid, FD_valid_state; intros; eauto.
+    - unfold refines_related;
+    apply SelfSimulation_Exists_change_owner.
+Qed.
+
+Theorem ss_AD_create:
+  forall n u u' v,
+    SelfSimulation u 
+    (FileDisk.refinement.(Simulation.Definitions.compile) (FileDiskOp.(Op) (Create v))) 
+    (FileDisk.refinement.(Simulation.Definitions.compile) (FileDiskOp.(Op) (Create v))) 
+    (FileDisk.refinement.(Simulation.Definitions.compile) (FileDiskOp.(Op) Recover)) AD_valid_state 
+    (AD_related_states u' None) (eq u') (authenticated_disk_reboot_list n).
+Proof.
+    intros; eapply SS_transfer.
+    - apply ss_FD_create.
+    - apply create_simulation.
+    - apply create_simulation.
+    - apply abstract_oracles_exist_wrt_create.
+    - apply abstract_oracles_exist_wrt_create.
+    - apply ORS_create.
+    - unfold exec_compiled_preserves_validity,
+    refines_valid, FD_valid_state; intros; eauto.
+    - unfold exec_compiled_preserves_validity,
+    refines_valid, FD_valid_state; intros; eauto.
+    - unfold refines_related;
+    apply SelfSimulation_Exists_create.
+Qed.
+
+
+Theorem ss_AD_delete:
+  forall n inum u u',
+    SelfSimulation u 
+    (FileDisk.refinement.(Simulation.Definitions.compile) (FileDiskOp.(Op) (Delete inum))) 
+    (FileDisk.refinement.(Simulation.Definitions.compile) (FileDiskOp.(Op) (Delete inum))) 
+    (FileDisk.refinement.(Simulation.Definitions.compile) (FileDiskOp.(Op) Recover)) AD_valid_state 
+    (AD_related_states u' None) (eq u') (authenticated_disk_reboot_list n).
+Proof.
+    intros; eapply SS_transfer.
+    - apply ss_FD_delete.
+    - apply delete_simulation.
+    - apply delete_simulation.
+    - apply abstract_oracles_exist_wrt_delete.
+    - apply abstract_oracles_exist_wrt_delete.
+    - apply ORS_delete.
+    - unfold exec_compiled_preserves_validity,
+    refines_valid, FD_valid_state; intros; eauto.
+    - unfold exec_compiled_preserves_validity,
+    refines_valid, FD_valid_state; intros; eauto.
+    - unfold refines_related;
+    apply SelfSimulation_Exists_delete.
+Qed.
+
+Theorem ss_AD_write_input:
+  forall n inum off u u' v1 v2,
+    SelfSimulation u 
+    (FileDisk.refinement.(Simulation.Definitions.compile) (FileDiskOp.(Op) (Write inum off v1))) 
+    (FileDisk.refinement.(Simulation.Definitions.compile) (FileDiskOp.(Op) (Write inum off v2))) 
+    (FileDisk.refinement.(Simulation.Definitions.compile) (FileDiskOp.(Op) Recover)) AD_valid_state 
+    (AD_related_states u' (Some inum)) (eq u') (authenticated_disk_reboot_list n).
+Proof.
+    intros; eapply SS_transfer.
+    - apply ss_FD_write_input.
+    - apply write_simulation.
+    - apply write_simulation.
+    - apply abstract_oracles_exist_wrt_write.
+    - apply abstract_oracles_exist_wrt_write.
+    - apply ORS_write_input.
+    - unfold exec_compiled_preserves_validity,
+    refines_valid, FD_valid_state; intros; eauto.
+    - unfold exec_compiled_preserves_validity,
+    refines_valid, FD_valid_state; intros; eauto.
+    - unfold refines_related; apply SelfSimulation_Exists_write_input.
+Qed.
+
+Theorem ss_AD_extend_input:
+  forall n inum u u' v1 v2,
+    SelfSimulation u 
+    (FileDisk.refinement.(Simulation.Definitions.compile) (FileDiskOp.(Op) (Extend inum v1))) 
+    (FileDisk.refinement.(Simulation.Definitions.compile) (FileDiskOp.(Op) (Extend inum v2))) 
+    (FileDisk.refinement.(Simulation.Definitions.compile) (FileDiskOp.(Op) Recover)) AD_valid_state 
+    (AD_related_states u' (Some inum)) (eq u') (authenticated_disk_reboot_list n).
+Proof.
+    intros; eapply SS_transfer.
+    - apply ss_FD_extend_input.
+    - apply extend_simulation.
+    - apply extend_simulation.
+    - apply abstract_oracles_exist_wrt_extend.
+    - apply abstract_oracles_exist_wrt_extend.
+    - apply ORS_extend.
+    - unfold exec_compiled_preserves_validity,
+    refines_valid, FD_valid_state; intros; eauto.
+    - unfold exec_compiled_preserves_validity,
+    refines_valid, FD_valid_state; intros; eauto.
+    - unfold refines_related; apply SelfSimulation_Exists_extend_input.
+Qed.
