src/Noninterference/TransactionalDisk/TransferProofs.v
@@ -1,0 +1,105 @@
+Require Import Framework FSParameters FileDiskLayer. (* LoggedDiskLayer TransactionCacheLayer TransactionalDiskLayer. *)
+Require Import TransactionalDiskRefinement FileDisk.TransferProofs FileDiskNoninterference ATCLayer.
+
+(* Notation "'TransactionalDiskCore'" := (TransactionalDiskOperation data_length). *)
+
+Fixpoint horizontally_compose_valid_prog1 {O1 O2} (L1: Language O1) (L2: Language O2) (LL: Language (HorizontalComposition O1 O2)) {T} (p1: prog L1 T) :=
+         match p1 with
+         | @Op _ T' p => Op (HorizontalComposition O1 O2) (P1 p)
+         | @Ret _ T' t => Ret t
+         | @Bind _ T1 T2 p1 p2 =>
+           Bind (horizontally_compose_valid_prog1 L1 L2 LL p1)
+           (fun r => horizontally_compose_valid_prog1 L1 L2 LL (p2 r))
+         end.
+
+
+Fixpoint horizontally_compose_valid_prog2 {O1 O2} (L1: Language O1) (L2: Language O2) (LL: Language (HorizontalComposition O1 O2)) {T} (p2: prog L2 T) :=
+         match p2 with
+         | @Op _ T' p => (Op (HorizontalComposition O1 O2) (P2 p))
+         | @Ret _ T' t => (Ret t)
+         | @Bind _ T1 T2 p1 p2 =>
+         Bind (horizontally_compose_valid_prog2 L1 L2 LL p1)
+         (fun r => horizontally_compose_valid_prog2 L1 L2 LL (p2 r))
+       end.
+
+
+Lemma ss_hc_rev_p1:
+  forall O1 O2 (L1: Language O1) (L2: Language O2) (LL: Language (HorizontalComposition O1 O2))
+    u R C V T l_grs1 l_grs2 (p1 p2: L1.(prog) T) rec,
+    @SelfSimulation _ LL u _ (horizontally_compose_valid_prog1 L1 L2 LL p1)
+    (horizontally_compose_valid_prog1 L1 L2 LL p2)
+    (horizontally_compose_valid_prog1 L1 L2 LL rec) R V  C l_grs2 ->
+    forall s2,
+      SelfSimulation u p1 p2 rec
+        (fun s1 => R (s1, s2))
+        (fun s1 s1' =>  V (s1, s2) (s1', s2))
+        C
+        l_grs1.
+Proof. Admitted.
+
+
+Lemma ss_hc_rev_p2:
+  forall O1 O2 (L1: Language O1) (L2: Language O2) (LL: Language (HorizontalComposition O1 O2))
+    u R C V T l_grs1 l_grs2 (p1 p2: L2.(prog) T) rec,
+    @SelfSimulation _ LL u _ (horizontally_compose_valid_prog2 L1 L2 LL p1)
+    (horizontally_compose_valid_prog2 L1 L2 LL p2)
+    (horizontally_compose_valid_prog2 L1 L2 LL rec) R V  C l_grs2 ->
+    forall s1,
+      SelfSimulation u p1 p2 rec
+        (fun s2 => R (s1, s2))
+        (fun s2 s2' =>  V (s1, s2) (s1, s2'))
+        C
+        l_grs1.
+Proof. Admitted.
+
+
+(*
+Theorem ss_TD_read:
+  forall n a u u' s,
+    @SelfSimulation _ TransactionalDisk u _
+    (TransactionalDiskCore.(Op) (Read a))
+    (TransactionalDiskCore.(Op) (Read a)) 
+    (TransactionalDiskCore.(Op) Recover) (TD_valid_state s) 
+    (TD_related_states u' None s) (eq u') (transactional_disk_reboot_list n).
+Proof.
+    intros.
+    eapply ss_hc_rev_p2 with (R:= AD_valid_state) (V:= AD_related_states u' None).
+    simpl; 
+    - apply ss_FD_read.
+    - apply read_simulation.
+    - apply read_simulation.
+    - apply abstract_oracles_exist_wrt_read.
+    - apply abstract_oracles_exist_wrt_read.
+    - apply ORS_read.
+    - unfold exec_compiled_preserves_validity,
+    refines_valid, FD_valid_state; intros; eauto.
+    - unfold exec_compiled_preserves_validity,
+    refines_valid, FD_valid_state; intros; eauto.
+    - unfold refines_related; apply SelfSimulation_Exists_read.
+Qed.
+*)
+
+Import FileDiskLayer.
+
+Theorem ss_ATC_read:
+  forall n inum off u u',
+    SelfSimulation u 
+    (compile (FileDisk.refinement.(Simulation.Definitions.compile) (FileDiskOp.(Op) (Read inum off)))) 
+    (compile (FileDisk.refinement.(Simulation.Definitions.compile) (FileDiskOp.(Op) (Read inum off)))) 
+    (compile (FileDisk.refinement.(Simulation.Definitions.compile) (FileDiskOp.(Op) Recover))) 
+    ATC_valid_state 
+    (ATC_related_states u' None) (eq u') (ATC_reboot_list n).
+Proof.
+    intros; eapply SS_transfer.
+    - apply ss_FD_read.
+    - apply read_simulation.
+    - apply read_simulation.
+    - apply abstract_oracles_exist_wrt_read.
+    - apply abstract_oracles_exist_wrt_read.
+    - apply ORS_read.
+    - unfold exec_compiled_preserves_validity,
+    refines_valid, FD_valid_state; intros; eauto.
+    - unfold exec_compiled_preserves_validity,
+    refines_valid, FD_valid_state; intros; eauto.
+    - unfold refines_related; apply SelfSimulation_Exists_read.
+Qed.
